Purely functional inlining done.

coq/Imp.v
@@ -121,6 +121,21 @@ Definition do_assn defs assn st : {prob state} :=
   sample: vals <- mapm_p id assn;
   dirac (updm st (mapm (feval_zexpr defs st) vals)).
 
+Lemma do_assnP defs assn st st' v :
+  st' \in supp (do_assn defs assn st) ->
+  if assn v is Some p then
+    exists2 e, e \in supp p & st' v = feval_zexpr defs st e
+  else st' v = st v.
+Proof.
+case/supp_sampleP=> /= vals /supp_mapm_pP [ed valsP] /supp_diracP {st'}->.
+rewrite updmE mapmE.
+case assn_v: (assn v)=> [p|].
+  have /dommP [e vals_v]: v \in domm vals by rewrite -ed mem_domm assn_v.
+  have e_p := valsP _ _ _ assn_v vals_v.
+  by exists e=> //; rewrite vals_v /=.
+by have /dommPn -> /=: v \notin domm vals by rewrite -ed mem_domm assn_v.
+Qed.
+
 Lemma do_assn0 defs st : do_assn defs emptym st = dirac st.
 Proof.
 rewrite /do_assn mapm_p0 sample_diracL; congr dirac.
@@ -222,396 +237,285 @@ apply/eq_ffun=> v; rewrite !(updmE, mapmE).
 case dassn_v: (dassn v)=> [e|] //=.
 *)
 
+Fixpoint com_mod_vars c : {fset var} :=
+  match c with
+  | CSkip => fset0
+  | CAssn assn c => domm assn :|: com_mod_vars c
+  | CIf _ cthen celse c => com_mod_vars cthen :|: com_mod_vars celse :|: com_mod_vars c
+  | CBlock vs block c => (com_mod_vars block :\: vs) :|: com_mod_vars c
+  end.
+
+Lemma com_mod_varsP defs c st st' v :
+  st' \in supp (run defs c st) ->
+  v \notin com_mod_vars c ->
+  st' v = st v.
+Proof.
+elim: c st st'.
+- by move=> /= st st' /supp_diracP ->.
+- move=> /= assn c IH st st''.
+  case/supp_sampleP=> st' /do_assnP-/(_ v).
+  rewrite in_fsetU negb_or mem_domm.
+  by case assn_v: (assn v)=> //= <-; eauto.
+- move=> /= e cthen IHthen celse IHelse c IH st st''.
+  case/supp_sampleP=> st' st'_supp st''_supp.
+  rewrite !in_fsetU !negb_or -andbA; case/and3P=> cthenP celseP cP.
+  rewrite (IH _ _ st''_supp) //.
+  by case: (feval_bexpr defs st e) st'_supp=> ?; eauto.
+- move=> /= vs block IHblock c IHc st st''.
+  case/supp_sampleP=> st' st'_supp st''_supp.
+  rewrite in_fsetU in_fsetD negb_or; case/andP=> v_mod v_c.
+  rewrite (IHc _ _ st''_supp v_c) updmE mkfmapfE mkffunE.
+  case: (boolP (v \in vs)) v_mod=> //= v_vs v_block.
+  by rewrite (IHblock _ _ st'_supp v_block) updmE mkfmapfE (negbTE v_vs).
+Qed.
+
 Module Inlining.
 
 Module Type CONFLICTS.
 Parameter conflicts :
-  renaming -> {fset var} -> {fset var}.
+  subst -> {fset var} -> {fset var}.
 Parameter conflicts_sub :
-  forall rn vs, fsubset vs (conflicts rn vs).
+  forall σ vs, fsubset vs (conflicts σ vs).
 Parameter conflicts_dis :
-  forall rn vs v,
-  v \in supp rn -> v \notin conflicts rn vs ->
-  fdisjoint (zexpr_vars (rn v)) (conflicts rn vs).
+  forall σ vs v,
+  v \in supp σ -> v \notin conflicts σ vs ->
+  fdisjoint (zexpr_vars [::] (σ v)) (conflicts σ vs).
 End CONFLICTS.
 
 Module Export Conflicts : CONFLICTS.
 
-Definition conflicts rn vs := supp rn :|: vs.
+Definition conflicts σ vs := supp σ :|: vs.
 
-Lemma conflicts_sub rn vs : fsubset vs (conflicts rn vs).
+Lemma conflicts_sub σ vs : fsubset vs (conflicts σ vs).
 Proof. exact: fsubsetUr. Qed.
 
-Lemma conflicts_dis rn vs v :
-  v \in supp rn -> v \notin conflicts rn vs ->
-  fdisjoint (zexpr_vars (rn v)) (conflicts rn vs).
+Lemma conflicts_dis σ vs v :
+  v \in supp σ -> v \notin conflicts σ vs ->
+  fdisjoint (zexpr_vars [::] (σ v)) (conflicts σ vs).
 Proof. by rewrite /conflicts in_fsetU => ->. Qed.
 
 End Conflicts.
 
-Inductive checkpoint_spec rn vs : renaming * renaming -> Prop :=
-| CheckpointSpec rn1 rn2 of
-  (forall st, flush id st (val rn) =
-    flush id (flush id st (val rn1)) (val rn2)) &
-  fdisjoint (supp rn2) vs &
-  (forall v, v \in supp rn2 -> fdisjoint (zexpr_vars (rn2 v)) vs)
-  : checkpoint_spec rn vs (rn1, rn2).
+Fixpoint inline_loop σ c : subst * com :=
+  match c with
+  | CSkip => (σ, CSkip)
+  | CAssn assn c =>
+    let assn := subst_assn σ assn in
+    let det_assn := filter_map (fun=> of_dirac) assn in
+    let cs := conflicts σ (domm assn) in
+    let σ_def v := if v \in cs then ZSym v
+                   else if det_assn v is Some e then e
+                   else σ v in
+    let σ := mkffun σ_def (domm det_assn :|: supp σ) in
+    let: (σ, c) := inline_loop σ c in
+    (σ, Assn assn;; c)
+  | CIf e cthen celse c =>
+    let e' := subst_bexpr (app_subst σ) e in
+    let: (σ_then, cthen') := inline_loop σ cthen in
+    let: (σ_else, celse') := inline_loop σ celse in
+    let modified := com_mod_vars cthen' :|: com_mod_vars celse' in
+    let can_merge := fdisjoint (bexpr_vars [::] e') modified in
+    let σ_def v := if can_merge then ZTest e' (σ_then v) (σ_else v)
+                   else if σ_then v == σ_else v then σ_then v
+                   else ZSym v in
+    let σ := mkffun σ_def (supp σ_then :|: supp σ_else) in
+    let: (σ, c) := inline_loop σ c in
+    (σ, CIf e' cthen' celse' c)
+  | CBlock vs block c =>
+    let cs := conflicts σ vs in
+    let σ_def v := if v \in cs then ZSym v else σ v in
+    let σ := mkffun σ_def (supp σ) in
+    let: (σ, block) := inline_loop σ block in
+    let cs := conflicts σ vs in
+    let σ_def v := if v \in cs then ZSym v else σ v in
+    let σ := mkffun σ_def (supp σ) in
+    let: (σ, c) := inline_loop σ c in
+    (σ, CBlock vs block c)
+  end.
 
-Module Type CHECKPOINT.
-Parameter checkpoint :
-  renaming -> {fset var} -> renaming * renaming.
-Parameter checkpointP :
-  forall rn vs, checkpoint_spec rn vs (checkpoint rn vs).
-End CHECKPOINT.
+Definition wf_subst defs σ st :=
+  forall v, feval_zexpr defs st (σ v) = st v.
 
-Module Export Checkpoint : CHECKPOINT.
-
-Definition checkpoint rn vs : renaming * renaming :=
-  let flush := conflicts rn vs in
-  let rn1   := mkffun rn flush in
-  let rn2   := mkffun rn (supp rn :\: flush) in
-  (rn1, rn2).
-
-Lemma checkpointP rn vs : checkpoint_spec rn vs (checkpoint rn vs).
+Lemma wf_subst_feval_zexpr σ st defs e :
+  wf_subst defs σ st ->
+  feval_zexpr defs st (subst_zexpr (app_subst σ) e) = feval_zexpr defs st e.
 Proof.
-exists.
-- move=> st; apply/eq_ffun=> /= v; rewrite !flushER mkffunE.
-  rewrite in_fsetD; case: (boolP (v \in conflicts rn vs))=> vc /=.
-    by rewrite flushER mkffunE vc.
-  case: ifPn=> vrn /= .
-    apply/(@eq_in_eval_zexprP (zexpr_vars (rn v))); rewrite ?fsubsetxx //.
-    move=> v' v'v; rewrite flushER mkffunE.
-    by move: (fdisjointP (conflicts_dis vrn vc) _ v'v)=> /negbTE ->.
-  by rewrite flushER mkffunE (negbTE vc) (suppPn vrn).
-- apply/fdisjointP=> v; rewrite mem_supp mkffunE in_fsetD.
-  case: (boolP (v \in conflicts rn vs)); rewrite /= ?eqxx //.
-  move=> vc _; apply: contra vc.
-  exact: (fsubsetP (conflicts_sub rn vs)).
-- move=> v; rewrite mem_supp mkffunE in_fsetD.
-  case: ifP; rewrite ?eqxx //.
-  case/andP=> vc vrn e; apply/fdisjointP=> v' v'v.
-  have {}v'v: v' \notin conflicts rn vs.
-    exact: (fdisjointP (conflicts_dis vrn vc)).
-  apply: contra v'v; exact: (fsubsetP (conflicts_sub rn vs)).
+move=> wf; rewrite /feval_zexpr subst_zexprP.
+apply/eq_eval_zexpr; case=> [v|s] //=; exact: wf.
 Qed.
 
-End Checkpoint.
-
-Fixpoint inline_loop rn c : renaming * com :=
-  match c with
-  | CSkip => (rn, CSkip)
-  | CAssn assn c =>
-    let det_assn := filter_map (fun=> of_dirac) assn in
-    if domm det_assn == domm assn then
-      let assn' := mapm (subst_zexpr rn) det_assn in
-      let rn'   := updm rn assn' in
-      inline_loop rn' c
-    else
-      let: (rn0, rn1) := checkpoint rn (domm assn) in
-      let: (rn2, c') :=  inline_loop rn1 c in
-      let  assn' := mapm (subst_zexpr rn1) assn in
-      (rn2, DAssn (val rn0);; Assn assn';; c')
-  | CIf e cthen celse c =>
-    let e' := subst_bexpr rn e in
-    let: (rn_then, cthen') := inline_loop rn cthen in
-    let: (rn_else, celse') := inline_loop rn celse in
-    let to_flush0 := supp rn_then :|: supp rn_else in
-    let updated v := (rn_then v != rn v) || (rn_else v != rn v) in
-    let to_flush1 := fset_filter updated to_flush0 in
-    if (cthen' == CSkip) && (celse' == CSkip) then
-      let merge v := ZTest e' (rn_then v) (rn_else v) in
-      let assn' := mkfmapf merge to_flush1 in
-      let rn' := updm rn assn' in
-      inline_loop rn' c
-    else
-      let assn_then := mkfmapf (dirac \o rn_then) to_flush1 in
-      let cthen''   := Seq cthen' (CAssn assn_then CSkip) in
-      let assn_else := mkfmapf (dirac \o rn_else) to_flush1 in
-      let celse''   := Seq celse' (CAssn assn_else CSkip) in
-      let rn_merge  := updm rn (mkfmapf ZVar to_flush1) in
-      let: (rn', c') := inline_loop rn_merge c in
-      (rn', CIf e' cthen'' celse'' c')
-  | CBlock vs block c =>
-    let: (rn0, rn1) := checkpoint rn vs in
-    let: (rn_block, block') := inline_loop rn1 block in
-    let: (rn2, rn3) := checkpoint rn_block vs in
-    let: (rn4, c') := inline_loop rn1 c in
-    (rn2, DAssn (val rn0);; Block vs (block';; DAssn (val rn2));; c')
-  end.
-
-Lemma inline_loopP rn c rn' c' st :
-  inline_loop rn c = (rn', c') ->
-  run id (DAssn (val rn);; c) st =
-  run id (c';; DAssn (val rn')) st.
+Lemma wf_subst_feval_bexpr σ st defs e :
+  wf_subst defs σ st ->
+  feval_bexpr defs st (subst_bexpr (app_subst σ) e) = feval_bexpr defs st e.
 Proof.
-elim: c rn c' rn' st.
-- by move=> rn _ _ st [<- <-] /=; rewrite Seqc1.
-- move=> assn c IH rn c' rn' st /=.
-  case: (altP (domm _ =P domm _))=> [e|_].
-  + set assn' := filter_map (fun=> of_dirac) assn in e.
-    have assnE : assn = mapm dirac assn'.
-      apply/eq_fmap=> v; move/eq_fset/(_ v): e.
-      rewrite !mem_domm /assn' mapmE filter_mapE.
-      case: (assn v)=> [pe|] //=.
-      by case: (of_dirac pe) (of_diracK pe)=> //= e ->.
-    move: assn' e assnE=> /= {}assn _ ->.
-    rewrite mapimK; last by move=> _; exact: diracK.
-    set rn0 := updm rn _; move=> {}/IH <-.
-    rewrite !run_DAssn -run_Assn run_DAssn; congr run.
-    apply/eq_ffun=> /= v.
-    rewrite !flushER flushE flushER /rn0 updmE mapmE.
-    case: (assn v)=> //= e.
-    by rewrite subst_zexprP; apply/eq_eval_zexpr=> v'; rewrite flushER.
-  + case: checkpointP=> rn0 rn1 chk1 chk2 chk3.
-    case e: (inline_loop rn1 c)=> [{}rn' {}c'] [<- <-].
-    move/IH in e.
-    rewrite run_DAssn -run_Assn chk1 -run_DAssn. -![in RHS]SeqA [RHS]run_DAssn.
-    rewrite -
+move=> wf; rewrite /feval_bexpr subst_bexprP.
+apply/eq_eval_bexpr; case=> [v|s] //=; exact: wf.
+Qed.
 
+Definition inline_loop_spec c :=
+  forall σ σ' c' st,
+    wf_subst [::] σ st ->
+    inline_loop σ c = (σ', c') ->
+    let p := run [::] c st in
+    run [::] c' st = p /\
+    forall st', st' \in supp p -> wf_subst [::] σ' st'.
 
-Lemma inline_loopP rn c st :
-  let res := inline_loop rn c in
-  run id c (flush st rn) =
-  sample: st' <- run id res.2 st;
-  dirac (flush st' res.1).
+Lemma inline_loop_skip : inline_loop_spec CSkip.
 Proof.
-elim: c rn st.
-- by move=> rn st; rewrite /= sample_diracL.
-- move=> assn c IH rn st /=.
-  case: (altP (domm _ =P domm _))=> [e|_].
-  + set assn' := filter_map (fun=> of_dirac) assn in e.
-    have assnE : assn = mapm dirac assn'.
-      apply/eq_fmap=> v; move/eq_fset/(_ v): e.
-      rewrite !mem_domm /assn' mapmE filter_mapE.
-      case: (assn v)=> [pe|] //=.
-      by case: (of_dirac pe) (of_diracK pe)=> //= e ->.
-    move: assn' e assnE=> /= {}assn _ ->.
-    rewrite mapm_p_comp.
-    under eq_mapm_p => ? do rewrite /= sample_diracL.
-    rewrite -(mapm_p_comp dirac (eval_zexpr (flush st rn))).
-    rewrite mapm_p_dirac sample_diracL mapimK; last first.
-      move=> _; exact: diracK.
-    by rewrite updm_flush IH.
-  + case: checkpointP=> rn0 rn1 chk1 chk2 chk3.
-    rewrite [inline_loop rn1 c]surjective_pairing /=.
-    rewrite -SeqA run_Seq assn_of_rnP sample_diracL.
+move=> σ _ _ st wf [<- <-]; split=> //= st'.
+by move=> /supp_diracP -> .
+Qed.
 
-
-
-    rewrite -mapm_mkfmapf mapm_p_comp.
-    under [in RHS]eq_mapm_p => /= e do rewrite sample_diracL.
-    set to_flush := conflicts rn (domm assn).
-    set assn0 := mkfmapf rn to_flush.
-    rewrite -[in RHS]mapm_p_comp mapm_p_dirac sample_diracL /= sampleA.
-    set rn0 := updm rn (mkfmapf ZVar to_flush).
-    set st0 := updm st (mapm (eval_zexpr st) assn0).
-    rewrite mapm_p_comp /=.
-    under [in RHS]eq_mapm_p => pe.
-      rewrite /= sampleA.
-      under eq_sample => e.
-        rewrite sample_diracL subst_zexprP.
-        under eq_eval_zexpr=> v.
-          rewrite (_ : eval_zexpr st0 (rn0 v) = flush st rn v); first over.
-          rewrite flushE /rn0 updmE mkfmapfE.
-          case: (boolP (v \in to_flush))=> [flush_v|not_flush_v].
-            by rewrite /= /st0 updmE mapmE /assn0 mkfmapfE flush_v /=.
-
-
-      over.
-    under [in RHS]eq_mapm_p => pe.
-      under eq_sample => e.
-
-
-Module Inlining.
-
-Notation renaming  := (ffun (fun v : var => v)).
-
-Record istate := IState {
-  fresh_vars  : ffun (fun n : string => 0 : nat);
-  formulas    : seq (var * zexpr);
-  (* Map formulas to the state variables needed to compute them. *)
-  used_vars   : ffun (fun v : var => fset1 v);
-}.
-
-Implicit Types (rn : renaming) (ist : istate).
-
-Definition state_view st rn ist :=
-  updm st (mkfmapf (eval_forms (formulas ist) st \o rn) (supp rn)).
-
-Definition istate_vars ist :=
-  \bigcup_(p <- formulas ist) (fset1 p.1 :|: zexpr_vars p.2) :|:
-  \bigcup_(v <- supp (used_vars ist)) used_vars ist v.
-
-Definition wf_istate ist :=
-  all (fun v => vnum v < fresh_vars ist (vname v)) (istate_vars ist).
-
-Definition M T : Type := istate → istate * T.
-
-Definition ret T (x : T) : M T :=
-  fun s => (s, x).
-
-Definition bind T S (x : M T) (f : T → M S) : M S :=
-  fun s => f (x s).2 (x s).1.
-
-Notation "'bind:' x '<-' t1 ';' t2" :=
-  (bind t1 (fun x => t2))
-  (at level 20, x pattern, t1 at level 100, t2 at level 200,
-   right associativity, format "'[' 'bind:'  x  '<-'  '[' t1 ;  ']' ']' '/' t2").
-
-Notation "f >> g" :=
-  (bind f (fun _ => g))
-  (at level 40, left associativity).
-
-Definition get T (f : istate → T) : M T :=
-  fun ist => (ist, f ist).
-
-Definition mod (f : istate → istate) : M unit :=
-  fun ist => (f ist, tt).
-
-Definition intern1 (rn : renaming) (v : var) (e : zexpr) : M renaming := fun ist =>
-  let: IState fv fs uv := ist in
-  let n   := vname v in
-  let vn  := fv n in
-  let v'  := Var n vn in
-  let fv' := upd fv n vn.+1 in
-  let e'  := subst_zexpr (ZVar \o rn) e in
-  let fs' := (v', e') :: fs in
-  let vs  := \bigcup_(v'' <- zexpr_vars e) uv v'' in
-  let uv' := upd uv v' vs in
-  let rn' := upd rn v v' in
-  (IState fv' fs' uv', rn').
-
-Lemma intern1P rn v e ist ist' rn' st v' :
-  intern1 rn v e ist = (ist', rn') ->
-  eval_forms (formulas ist') st (rn' v') =
-  if v' == v then
-    eval_zexpr (eval_forms (formulas ist') st) e
-  else eval_forms (formulas ist') st (rn v).
+Lemma inline_loop_assn assn c :
+  inline_loop_spec c ->
+  inline_loop_spec (CAssn assn c).
 Proof.
-case: ist=> fv fs uv /= [<- <-] {ist' rn'} /=.
-rewrite updE; case: (altP (v' =P v))=> [_|ne].
-  rewrite eqxx subst_zexprP; apply: eq_eval_zexpr=> v'' /=.
+move=> IH σ σ'' c'' st /=.
+set assn' := subst_assn σ assn.
+set det_assn := filter_map _ _.
+set cs := conflicts σ _.
+set σ'_def := fun v => if v \in cs then ZSym v else _.
+set σ' := mkffun _ _.
+case ec: inline_loop => [{}σ'' {}c''] wf [<- <-] /=.
+rewrite run_Assn /=.
+have -> : do_assn [::] assn' st = do_assn [::] assn st.
+  rewrite /do_assn /assn' /subst_assn mapm_p_comp /=.
+  rewrite mapm_p_sample sampleA; apply/eq_sample=> /= vals.
+  rewrite -mapm_p_comp mapm_p_dirac sample_diracL -mapm_comp.
+  by under eq_mapm=> /= e do rewrite wf_subst_feval_zexpr //.
+set p_st' := do_assn [::] assn st.
+suff wf' st' : st' \in supp p_st' -> wf_subst [::] σ' st'.
+  split.
+    by apply/eq_in_sample=> st' {}/wf' wf'; case: (IH _ _ _ _ wf' ec).
+  move=> st'' /supp_sampleP [st' {}/wf' wf'].
+  case: (IH _ _ _ _ wf' ec)=> _; exact.
+move=> st'P.
+have st_cs v: v \notin cs -> st' v = st v.
+  move=> v_cs; have: v \notin domm assn'.
+    apply: contra v_cs; apply/fsubsetP/conflicts_sub.
+  rewrite domm_map=> vP.
+  case/supp_sampleP: st'P=> /= exps /supp_mapm_pP [ed _] /supp_diracP ->.
+  rewrite updmE mapmE; move: vP; rewrite ed mem_domm.
+  by case: (exps v).
+move=> v; rewrite /σ' mkffunE; case: ifP=> // v_domm.
+rewrite /σ'_def; case: ifPn=> // v_cs.
+have /dommPn det_v: v \notin domm det_assn.
+  apply: contra v_cs; apply/fsubsetP.
+  apply: fsubset_trans (conflicts_sub _ _).
+  by rewrite domm_filter_map fset_filter_subset.
+rewrite in_fsetU mem_domm det_v /= in v_domm *.
+have dis : fdisjoint (zexpr_vars [::] (σ v)) cs by exact: conflicts_dis.
+rewrite st_cs // -wf; apply: eq_in_feval_zexpr => v' in_σ_v.
+apply: st_cs; exact: (fdisjointP dis).
+Qed.
 
-Definition intern (rn : renaming) (assn : {fmap var -> zexpr}) : M renaming :=
-  foldl (fun f ve => bind: rn' <- f; intern1 rn' ve.1 ve.2) (ret rn) (val assn).
-
-Definition conflicts (rn : renaming) (vs : {fset var}) : M {fset var} := fun ist =>
-  let: IState fv fs uv := ist in
-  (IState fv fs uv,
-   fset_filter (fun v => fdisjoint (uv (rn v)) vs) (supp rn)).
-
-Fixpoint inline_loop (rn : renaming) (c : com) : M (renaming * com) :=
-  match c with
-  | CSkip =>
-    ret (rn, CSkip)
-  | CAssn assn c =>
-    let det_assn := filter_map (fun=> of_dirac) assn in
-    if domm det_assn == domm assn then
-      bind: rn' <- intern rn det_assn;
-      inline_loop rn' c
-    else
-      bind: to_flush <- conflicts rn (domm assn);
-      let assn0 := mkfmapf (dirac \o ZVar \o rn) to_flush in
-      let rn0   := updm rn (mkfmapf id to_flush) in
-      let assn1 := mapm (fun pe => sample: e <- pe; dirac (subst_zexpr (ZVar \o rn0) e)) assn in
-      let rn1   := updm rn0 (mkfmapf id (domm assn1)) in
-      bind: (rn', c') <- inline_loop rn c;
-      ret (rn', CAssn assn0 (CAssn assn1 c'))
-  | CIf e cthen celse c =>
-    let e' := subst_bexpr (ZVar \o rn) e in
-    bind: (rn_then, cthen') <- inline_loop rn cthen;
-    bind: (rn_else, celse') <- inline_loop rn celse;
-    let to_flush0 := supp rn_then :|: supp rn_else in
-    let updated v := (rn_then v != rn v) || (rn_else v != rn v) in
-    let to_flush1 := fset_filter updated to_flush0 in
-    match cthen', celse' with
-    | CSkip, CSkip =>
-      let merge v := ZTest e' (ZVar (rn_then v)) (ZVar (rn_else v)) in
-      bind: rn' <- intern rn (mkfmapf merge to_flush1);
-      inline_loop rn' c
-    | _, _ =>
-      let assn_then := mkfmapf (dirac \o ZVar \o rn_then) to_flush1 in
-      let cthen''   := Seq cthen' (CAssn assn_then CSkip) in
-      let assn_else := mkfmapf (dirac \o ZVar \o rn_else) to_flush1 in
-      let celse''   := Seq celse' (CAssn assn_else CSkip) in
-      let rn_merge  := updm rn (mkfmapf id to_flush1) in
-      bind: (rn', c') <- inline_loop rn_merge c;
-      ret (rn', CIf e' cthen'' celse'' c')
-    end
-  | CBlock vs c1 c2 =>
-    bind: to_flush0 <- conflicts rn vs;
-    let assn0 := mkfmapf (dirac \o ZVar \o rn) to_flush0 in
-    let rn0 := updm rn (mkfmapf id (to_flush0 :|: vs)) in
-    bind: (rn1, c1') <- inline_loop rn0 c1;
-    bind: to_flush1  <- conflicts rn1 vs;
-    let assn1 := mkfmapf (dirac \o ZVar \o rn1) to_flush1 in
-    let rn1'  := updm rn1 (mkfmapf id to_flush1) in
-    bind: (rn2, c2') <- inline_loop rn1' c2;
-    ret (rn2, CAssn assn0 (CBlock vs c1 c2))
-  end.
-
-Lemma inline_loopP rn rn' c c' ist ist' st :
-  inline_loop rn c ist = (ist', (rn', c')) ->
-  run id c (state_view st rn ist') =
-  sample: st' <- run (eval_forms (formulas ist')) c' st;
-  dirac (state_view st' rn' ist).
+Lemma inline_loop_if e cthen celse c :
+  inline_loop_spec cthen ->
+  inline_loop_spec celse ->
+  inline_loop_spec c ->
+  inline_loop_spec (CIf e cthen celse c).
 Proof.
-elim: c rn rn' c' ist ist' st.
-- move=> /= rn _ _ ist _ st [<- <- <-] /=.
-  by rewrite sample_diracL.
-- move=> /= assn c IH rn rn' c' ist ist' st.
-  set det_assn := filter_map _ _; case: ifP=> [/eqP edomm|_].
-  +
+move=> IHthen IHelse IHc σ σ'' c' st /=.
+case ethen: (inline_loop σ cthen)=> [σ_then cthen'].
+case eelse: (inline_loop σ celse)=> [σ_else celse'].
+set e' := subst_bexpr (app_subst σ) e.
+set cond := feval_bexpr [::] st e.
+set cb := if cond then cthen else celse.
+set cb' := if cond then cthen' else celse'.
+set can_merge := fdisjoint _ _.
+set σ'_def := fun v => if can_merge then _ else _.
+set σ' := mkffun σ'_def (supp σ_then :|: supp σ_else).
+set σ_b := if cond then σ_then else σ_else.
+have {IHthen IHelse} IHb : inline_loop_spec cb.
+  rewrite /cb; case: (cond); [exact: IHthen|exact: IHelse].
+have eb : inline_loop σ cb = (σ_b, cb').
+  by rewrite /cb /σ_b /cb'; case: (cond).
+case ec: (inline_loop σ' c)=> [{}σ'' {}c'] wf [<- <-] /=.
+rewrite wf_subst_feval_bexpr // -/cond -/cb'.
+case/(_ _ _ _ _ wf eb): IHb=> ecb wf'.
+suff wf'' st' : st' \in supp (run [::] cb st) -> wf_subst [::] σ' st'.
+  split.
+    rewrite ecb; apply/eq_in_sample=> st' {}/wf'' wf''.
+    by case/(_ _ _ _ _ wf'' ec): IHc.
+  move=> st'' /supp_sampleP [st' {}/wf'' wf'' st''_supp].
+  case/(_ _ _ _ _ wf'' ec): IHc=> _; exact.
+move=> st'_supp v; move/(_ _ st'_supp v) in wf'.
+rewrite -wf' /σ' mkffunE; case: ifPn=> [_|]; last first.
+  rewrite in_fsetU negb_or; case/andP=> /suppPn v_then /suppPn v_else.
+  by rewrite /σ_b; case: (cond); rewrite ?v_then ?v_else.
+rewrite /σ'_def /σ_b /=; case: (boolP can_merge)=> [dis|_].
+  have {}dis: fdisjoint (bexpr_vars [::] e') (com_mod_vars cb').
+    move: dis; rewrite /can_merge fdisjointUr; case/andP.
+    by rewrite /cb'; case: (cond).
+  pose cond' := feval_bexpr [::] st' e'.
+  pose ev e := feval_zexpr [::] st' e.
+  rewrite -[LHS]/(if cond' then ev (σ_then v) else ev (σ_else v)).
+  have ->: cond' = feval_bexpr [::] st e'.
+    apply/eq_in_feval_bexpr=> v' /(fdisjointP dis).
+    move: st'_supp; rewrite -ecb; exact: com_mod_varsP.
+  by rewrite wf_subst_feval_bexpr // /cond; case: feval_bexpr.
+case: eqP=> [?|_]; first by case: (cond)=> //; congruence.
+by rewrite wf'.
+Qed.
 
-Definition spec T (P : istate → Prop) (x : M T) (Q : T → istate → Prop) : Prop :=
-  ∀ s, P s → Q (x s).2 (x s).1.
-
-
-
-
-
-
-
-
-
-Fixpoint com_read_vars c : {fset var} :=
-  match c with
-  | Skip =>
-    fset0
-  | Assn assn c =>
-    assn_vars assn :|: com_read_vars c
-  | If be cthen celse c =>
-    bexpr_vars be :|:
-    com_read_vars cthen :|:
-    com_read_vars celse :|:
-    com_read_vars c
-  | Block vs block c =>
-    (com_read_vars block :\: vs) :|:
-    com_read_vars c
-  end.
-
-Lemma com_read_varsP (V : {fset var}) c st1 st2 :
-  {in V, st1 =1 st2} ->
-  fsubset (com_read_vars c) V ->
-  forall st1', st1' \in supp (run c st1) ->
-  forall st2', st2' \in supp (run c st2) ->
-  {in V, st1' =1 st2'}.
+Lemma inline_loop_block vs block c :
+  inline_loop_spec block ->
+  inline_loop_spec c ->
+  inline_loop_spec (CBlock vs block c).
 Proof.
-elim: c st1 st2=> //=.
-- by move=> ??? _ _ /supp_diracP -> _ /supp_diracP ->.
-- move=> assn c IH st1 st2 e.
-  rewrite fsubUset; case/andP=> sub_c sub_assn.
-  move=> st1' /supp_sampleP [/= vals1 vals1P st1'P].
-  move=> st2' /supp_sampleP [/= vals2 vals2P st2'P].
-  have {}e: {in V, upd st1 vals1 =1 upd st2 vals2}.
-    admit.
-  by apply: IH; eauto.
-- move=> be cthen IHthen celse IHelse c IH st1 st2 e.
-  rewrite !fsubUset -!andbA; case/and4P=> sub_be sub_cthen sub_celse sub_c.
-  move=> st1'' /supp_sampleP [/= st1' st1'P st1''P].
-  move=> st2'' /supp_sampleP [/= st2' st2'P st2''P].
-  rewrite -(bexpr_varsP e sub_be) in st2'P.
-  suff ?: {in V, st1' =1 st2'} by eauto using IH.
-  case: eval_bexpr in st1'P st2'P.
-  + by eauto using IHthen.
-  + by eauto using IHelse.
+move=> IHblock IHc σ0 σ4 c' st0 wf0 /=.
+set cs0 := conflicts σ0 vs.
+set σ1_def := fun v => if v \in cs0 then ZSym v else σ0 v.
+set σ1 := mkffun σ1_def (supp σ0).
+case eblock: (inline_loop σ1 block)=> [σ2 block'].
+set cs2 := conflicts σ2 vs.
+set σ3_def := fun v => if v \in cs2 then ZSym v else σ2 v.
+set σ3 := mkffun σ3_def (supp σ2).
+case ec: (inline_loop σ3 c)=> [{}σ4 {}c'] [<- <-] /=.
+set st1 := updm st0 (mkfmapf (fun=> 0%R) vs).
+have wf1 : wf_subst [::] σ1 st1.
+  move=> v; rewrite /σ1 /σ1_def mkffunE.
+  case: ifPn=> //= v_σ0; case: ifPn=> //= v_cs0.
+  have v_vs : v \notin vs.
+    apply: contra v_cs0; apply/fsubsetP; exact: conflicts_sub.
+  rewrite /st1 updmE mkfmapfE (negbTE v_vs).
+  rewrite -wf0; apply/eq_in_feval_zexpr=> v' v'_v.
+  rewrite updmE mkfmapfE.
+  have v'_cs0 : v' \notin cs0.
+    by move: v'_v; apply/fdisjointP; apply: conflicts_dis.
+  suff /negbTE -> : v' \notin vs by [].
+  apply: contra v'_cs0; apply/fsubsetP; exact: conflicts_sub.
+have [{}eblock wf2] := IHblock _ _ _ _ wf1 eblock.
+set r0 := mkfmapf (mkffun st0 vs) vs.
+have r0E v : r0 v = if v \in vs then Some (st0 v) else None.
+  by rewrite /r0 mkfmapfE mkffunE; case: ifP=> // ->.
+set p2 := run [::] block st1 in eblock *.
+have wf3 st2 : st2 \in supp p2 -> wf_subst [::] σ3 (updm st2 r0).
+  move=> {}/wf2 wf2 v; rewrite /σ3 /σ3_def mkffunE.
+  case: ifP=> //= v_σ2; case: ifPn=> // v_cs2.
+  have v_vs : v \notin vs.
+    apply: contra v_cs2; apply/fsubsetP; exact: conflicts_sub.
+  rewrite updmE r0E (negbTE v_vs) -wf2.
+  apply/eq_in_feval_zexpr=> v' v'_v.
+  have v'_cs2 : v' \notin cs2.
+    by move: v'_v; apply/fdisjointP; apply: conflicts_dis.
+  have v'_vs : v' \notin vs.
+    apply: contra v'_cs2; apply/fsubsetP; exact: conflicts_sub.
+  by rewrite updmE r0E (negbTE v'_vs).
+rewrite eblock; split.
+  apply/eq_in_sample=> st2 {}/wf3 wf3.
+  by have [{}ec wf4] := IHc _ _ _ _ wf3 ec.
+move=> st4 /supp_sampleP [st2 {}/wf3 wf3 st4_supp].
+have [_ wf4] := IHc _ _ _ _ wf3 ec; exact: wf4.
+Qed.
+
+Lemma inline_loopP c : inline_loop_spec c.
+Proof.
+elim: c=> *.
+- exact: inline_loop_skip.
+- exact: inline_loop_assn.
+- exact: inline_loop_if.
+- exact: inline_loop_block.
+Qed.
+
+End Inlining.
